support for arguments

src/3d/ocaml/Lisp.ml
@@ -25,20 +25,19 @@ let parse_witness = function
 let read_witness_from (from: unit -> string) =
   let (letbinding, sexp) = read_lisp_from from in
   let witness = parse_witness sexp in
-  print_string ";; witness: [";
-  List.iter (fun i -> print_string (Prims.to_string i); print_string "; ") witness;
-  print_endline "]";
   (letbinding, FStar_Seq_Properties.seq_of_list witness)
 
-let parse_int (name: string) = function
+let parse_any (name: string) = function
   | Sexplib.Sexp.List [Sexplib.Sexp.List [Sexplib.Sexp.Atom name'; Sexplib.Sexp.Atom n]]
     when name = name' ->
-    Prims.parse_int n
-  | _ -> failwith ("parse_int: "^name^" not found")
+    n
+  | _ -> failwith ("parse_any: "^name^" not found")
+
+let parse_int (name: string) sexp = Prims.parse_int (parse_any name sexp)
 
 let read_int_from (from: unit -> string) (name: string) =
   let (letbinding, sexp) = read_lisp_from from in
   (letbinding, parse_int name sexp)
 
-let read_any_from (from: unit -> string) : string =
-  fst (read_lisp_from from)
+let read_any_from (from: unit -> string) (name: string) : string =
+  parse_any name (snd (read_lisp_from from))
